SStructTT/Static/Inversion.lean
@@ -1,0 +1,7 @@
+import SStructTT.Static.Typed
+
+namespace Static
+variable {Srt : Type} [inst : SStruct Srt]
+
+-- lemma Typed.pi_inv {Γ : Ctx Srt} {A B C s} :
+--   Γ
